src/tools/parallelcomposition/translateTosapic/translate_to_sapicScript.sml
@@ -160,6 +160,24 @@ val sim_def = Define`
 
               
 
+val symbtree_to_sapic_initial_state_simulation_thm = store_thm(
+  "symbtree_to_sapic_initial_state_simulation_thm",
+  ``
+∀T0 C0 H0 Re0 NRe0.
+        (((val_of_tree T0) = SOME (Silent,0,H0)) ∧
+        (C0 = (Pconfig ((symbtree_to_sapic T0),0,Re0,NRe0)))∧
+        ((symb_interpr_dom H0) = {})∧
+        (sapic_renaming_dom Re0 = {}))
+         ⇒ (sim T0 C0)``,  
+rw[sim_def] >-(
+IMP_RES_TAC position_of_val_thm>>
+ASM_SIMP_TAC (srw_ss()) []
+)>>
+IMP_RES_TAC env_of_val_thm>>
+ASM_SIMP_TAC (srw_ss()) []
+)
+
+        
 val symbtree_to_sapic_single_step_simulation_thm = store_thm(
   "symbtree_to_sapic_single_step_simulation_thm",
   ``
@@ -409,11 +427,288 @@ ASM_SIMP_TAC (srw_ss()) []
 (*end of silent *)
 );
 
+        
+(*
+
+
+val trace_sim_def = Define`
+                   ( trace_sim Tev Pev =
+                   (∃tre tre' Pro i Re NRe Pro' i' Re' NRe'.
+                   (execute_symbolic_tree tre Tev tre')∧
+                   (sapic_position_multi_transitions (Pconfig (Pro,i,Re,NRe)) Pev (Pconfig (Pro',i',Re',NRe'))) ∧
+                     ((sim tre (Pconfig (Pro,i,Re,NRe))) ∧
+                       (sim tre' (Pconfig (Pro',i',Re',NRe'))) 
+                      )))
+`;       
+
+∀E Tree Tree' Pro i Re NRe.
+        (((execute_symbolic_tree Tree E Tree' ) ∧ (sim Tree (Pconfig (Pro,i,Re,NRe))))
+         ⇒ (∃Pro' i' Re' NRe' Ev. (sim Tree' (Pconfig (Pro',i',Re',NRe'))) ∧ (sapic_position_multi_transitions (Pconfig (Pro,i,Re,NRe)) Ev (Pconfig (Pro',i',Re',NRe')))))
+
+
+gen_tac>>
+  Cases_on ‘E’ >-(
+    rw[execute_symbolic_tree_def]>>
+    IMP_RES_TAC sapic_position_multi_transitions_def>>
+    FULL_SIMP_TAC (list_ss++pred_setSimps.PRED_SET_ss++boolSimps.LIFT_COND_ss++boolSimps.EQUIV_EXTRACT_ss) [sapic_position_multi_transitions_def]>>
+                  metis_tac[symbtree_to_sapic_initial_state_simulation_thm]
+)
+>-(
+rpt strip_tac
+IMP_RES_TAC execute_symbolic_tree_def
+FULL_SIMP_TAC (list_ss++pred_setSimps.PRED_SET_ss++boolSimps.LIFT_COND_ss++boolSimps.EQUIV_EXTRACT_ss) []
+IMP_RES_TAC sapic_position_multi_transitions_def
+FULL_SIMP_TAC (list_ss++pred_setSimps.PRED_SET_ss++boolSimps.LIFT_COND_ss++boolSimps.EQUIV_EXTRACT_ss) []
+IMP_RES_TAC symbtree_to_sapic_single_step_simulation_thm
+
+            metis_tac[symbtree_to_sapic_single_step_simulation_thm]
+
+)        
+)
 
 
 
 
+
+
+
+
+
+
+        
+val symbtree_to_sapic_single_step_simulation_thm = store_thm(
+  "symbtree_to_sapic_single_step_simulation_thm",
+  ``
+∀Tev Pev T0 Tree H0 Re0 NRe0 Pro i Re NRe.
+  ((val_of_tree T0 = SOME (Silent,0,H0))∧
+  (symb_interpr_dom H0 = ∅) ∧
+  (sapic_renaming_dom Re0 = ∅) ∧
+  (execute_symbolic_tree T0 Tev Tree) ∧ (sapic_position_multi_transitions (Pconfig ((symbtree_to_sapic T0),0,Re0,NRe0)) (MAP sbirEvent_to_sapicFact Tev) (Pconfig (Pro,i,Re,NRe))))
+  ⇒ (sim Tree (Pconfig (Pro,i,Re,NRe)))``,
+gen_tac>>
+  Cases_on ‘Tev’ >-(
+    rw[execute_symbolic_tree_def]>>
+    IMP_RES_TAC sapic_position_multi_transitions_def>>
+    FULL_SIMP_TAC (list_ss++pred_setSimps.PRED_SET_ss++boolSimps.LIFT_COND_ss++boolSimps.EQUIV_EXTRACT_ss) [sapic_position_multi_transitions_def]>>
+                  metis_tac[symbtree_to_sapic_initial_state_simulation_thm]
+)
+>-(
+rpt strip_tac
+IMP_RES_TAC execute_symbolic_tree_def
+FULL_SIMP_TAC (list_ss++pred_setSimps.PRED_SET_ss++boolSimps.LIFT_COND_ss++boolSimps.EQUIV_EXTRACT_ss) []
+IMP_RES_TAC sapic_position_multi_transitions_def
+FULL_SIMP_TAC (list_ss++pred_setSimps.PRED_SET_ss++boolSimps.LIFT_COND_ss++boolSimps.EQUIV_EXTRACT_ss) []
+IMP_RES_TAC symbtree_to_sapic_single_step_simulation_thm
+
+         
+
+val symbtree_to_sapic_single_step_simulation_thm = store_thm(
+  "symbtree_to_sapic_single_step_simulation_thm",
+  ``
+∀Tev Pev T0 Tree H0 Re0 NRe0 Pro i Re NRe.
+  ((sim T0 (Pconfig ((symbtree_to_sapic T0),0,Re0,NRe0)))∧
+  (execute_symbolic_tree T0 Tev Tree) ∧
+  (sapic_position_multi_transitions (Pconfig ((symbtree_to_sapic T0),0,Re0,NRe0)) (MAP sbirEvent_to_sapicFact Tev) (Pconfig (Pro,i,Re,NRe))))
+  ⇒ (sim Tree (Pconfig (Pro,i,Re,NRe)))``,
+gen_tac>>
+  Cases_on ‘Tev’ >-(
+    rw[execute_symbolic_tree_def]>>
+    IMP_RES_TAC sapic_position_multi_transitions_def>>
+    FULL_SIMP_TAC (list_ss++pred_setSimps.PRED_SET_ss++boolSimps.LIFT_COND_ss++boolSimps.EQUIV_EXTRACT_ss) [sapic_position_multi_transitions_def]>>
+                  metis_tac[symbtree_to_sapic_initial_state_simulation_thm]
+)
+>-(
+rpt strip_tac
+IMP_RES_TAC execute_symbolic_tree_def
+FULL_SIMP_TAC (list_ss++pred_setSimps.PRED_SET_ss++boolSimps.LIFT_COND_ss++boolSimps.EQUIV_EXTRACT_ss) []
+IMP_RES_TAC sapic_position_multi_transitions_def
+FULL_SIMP_TAC (list_ss++pred_setSimps.PRED_SET_ss++boolSimps.LIFT_COND_ss++boolSimps.EQUIV_EXTRACT_ss) []
+IMP_RES_TAC symbtree_to_sapic_single_step_simulation_thm
+
+            metis_tac[symbtree_to_sapic_single_step_simulation_thm]
+
+)        
+)
+
+
+
+
+
+
+
+
+
+
+        
+val symbtree_to_sapic_single_step_simulation_thm = store_thm(
+  "symbtree_to_sapic_single_step_simulation_thm",
+  ``
+∀Tev Pev T0 Tree H0 Re0 NRe0 Pro i Re NRe.
+  ((val_of_tree T0 = SOME (Silent,0,H0))∧
+  (symb_interpr_dom H0 = ∅) ∧
+  (sapic_renaming_dom Re0 = ∅) ∧
+  (execute_symbolic_tree T0 Tev Tree) ∧ (sapic_position_multi_transitions (Pconfig ((symbtree_to_sapic T0),0,Re0,NRe0)) (MAP sbirEvent_to_sapicFact Tev) (Pconfig (Pro,i,Re,NRe))))
+  ⇒ (sim Tree (Pconfig (Pro,i,Re,NRe)))``,
+gen_tac>>
+  Cases_on ‘Tev’ >-(
+    rw[execute_symbolic_tree_def]>>
+    IMP_RES_TAC sapic_position_multi_transitions_def>>
+    FULL_SIMP_TAC (list_ss++pred_setSimps.PRED_SET_ss++boolSimps.LIFT_COND_ss++boolSimps.EQUIV_EXTRACT_ss) [sapic_position_multi_transitions_def]>>
+                  metis_tac[symbtree_to_sapic_initial_state_simulation_thm]
+)
+>-(
+rpt strip_tac
+IMP_RES_TAC execute_symbolic_tree_def
+FULL_SIMP_TAC (list_ss++pred_setSimps.PRED_SET_ss++boolSimps.LIFT_COND_ss++boolSimps.EQUIV_EXTRACT_ss) []
+IMP_RES_TAC sapic_position_multi_transitions_def
+FULL_SIMP_TAC (list_ss++pred_setSimps.PRED_SET_ss++boolSimps.LIFT_COND_ss++boolSimps.EQUIV_EXTRACT_ss) []
+IMP_RES_TAC symbtree_to_sapic_single_step_simulation_thm
+PAT_X_ASSUM ``!i Re Pro NRe. A`` (ASSUME_TAC o (Q.SPECL [`i'`,`Re'`,`Pro'`,`NRe'`])) >>
+        RES_TAC
+)        
+)
+
+
+
+val symbtree_to_sapic_single_step_simulation_thm = store_thm(
+  "symbtree_to_sapic_single_step_simulation_thm",
+  ``
+∀Tev T0 Tree H0 Re0 NRe0.
+  ((execute_symbolic_tree T0 Tev Tree) ∧
+  (sim T0 (Pconfig ((symbtree_to_sapic T0),0,Re0,NRe0))))
+  ⇒
+  (∃Pro i Re NRe Pev. (sapic_position_multi_transitions (Pconfig ((symbtree_to_sapic T0),0,Re0,NRe0)) Pev (Pconfig (Pro,i,Re,NRe))) ∧
+  (sim Tree (Pconfig (Pro,i,Re,NRe))))``,
+gen_tac>>
+  Cases_on ‘Tev’ >-(
+    rw[execute_symbolic_tree_def]>>
+    Q.EXISTS_TAC `symbtree_to_sapic T0` >>
+    Q.EXISTS_TAC `0` >>
+    Q.EXISTS_TAC `Re0` >>
+    Q.EXISTS_TAC `NRe0` >>
+    Q.EXISTS_TAC `[]` >>
+    rw[sapic_position_multi_transitions_def]    
+)
+>-(
+rpt strip_tac
+IMP_RES_TAC execute_symbolic_tree_def
+FULL_SIMP_TAC (list_ss++pred_setSimps.PRED_SET_ss++boolSimps.LIFT_COND_ss++boolSimps.EQUIV_EXTRACT_ss) []
+IMP_RES_TAC symbtree_to_sapic_single_step_simulation_thm
+rewrite_tac[sapic_position_multi_transitions_def]
+    Q.EXISTS_TAC `Pro'` >>
+    Q.EXISTS_TAC `i'` >>
+    Q.EXISTS_TAC `Re'` >>
+    Q.EXISTS_TAC `NRe'` >>
+    Q.EXISTS_TAC `e::ev` >>
+    ASM_SIMP_TAC (srw_ss()) []
+)        
+)
+
+
+
+
+
+
+
+rpt strip_tac
+IMP_RES_TAC execute_symbolic_tree_def
+FULL_SIMP_TAC (list_ss++pred_setSimps.PRED_SET_ss++boolSimps.LIFT_COND_ss++boolSimps.EQUIV_EXTRACT_ss) []
+IMP_RES_TAC sapic_position_multi_transitions_def
+FULL_SIMP_TAC (list_ss++pred_setSimps.PRED_SET_ss++boolSimps.LIFT_COND_ss++boolSimps.EQUIV_EXTRACT_ss) []
+IMP_RES_TAC symbtree_to_sapic_single_step_simulation_thm
+metis_tac[symbtree_to_sapic_single_step_simulation_thm]
+PAT_X_ASSUM ``!i Re Pro NRe. A`` (ASSUME_TAC o (Q.SPECL [`i'`,`Re'`,`Pro'`,`NRe'`])) >>
+        RES_TAC
+        
+val TreeTransNil = new_axiom ("TreeTransNil",
+                            ``∀T e. (execute_symbolic_tree T e T) ⇒
+                            (e = [])``);        
+val PTransEq = new_axiom ("PTransEq",
+                            ``∀C C' e e'. (sapic_position_multi_transitions C e C') ∧ (sapic_position_multi_transitions C e' C') ⇒ (e = e')``);
+
+val TreeTransEq = new_axiom ("TreeTransEq",
+                            ``∀e e' T T'. (execute_symbolic_tree T e T') ∧ (execute_symbolic_tree T e' T') ⇒ (e = e')``
+                           gen_tac
+                           gen_tac
+Cases_on  ‘e = e'’                           
+metis_tac[]
+
+       Cases_on ‘e’
+       rpt strip_tac
+       IMP_RES_TAC execute_symbolic_tree_def
+       FULL_SIMP_TAC (list_ss++pred_setSimps.PRED_SET_ss++boolSimps.LIFT_COND_ss++boolSimps.EQUIV_EXTRACT_ss) []
+       metis_tac[TreeTransNil]
 
        
+       
+);
+                                                        
+val symbtree_to_sapic_single_step_simulation_thm = store_thm(
+  "symbtree_to_sapic_single_step_simulation_thm",
+  ``
+∀Tev Pev T0 Tree H0 Re0 NRe0 Pro i Re NRe.
+  ((execute_symbolic_tree T0 Tev Tree) ∧
+  (sapic_position_multi_transitions (Pconfig ((symbtree_to_sapic T0),0,Re0,NRe0)) (MAP sbirEvent_to_sapicFact Tev) (Pconfig (Pro,i,Re,NRe)))∧
+  (sim T0 (Pconfig ((symbtree_to_sapic T0),0,Re0,NRe0))))
+  ⇒ ((traces_of_sapic (Pconfig ((symbtree_to_sapic T0),0,Re0,NRe0)) (Pconfig (Pro,i,Re,NRe))) = IMAGE (MAP sbirEvent_to_sapicFact) (traces_of_tree T0 Tree))``,
+  rewrite_tac[traces_of_tree_def,traces_of_sapic_def,EXTENSION,IMAGE_DEF]
+  FULL_SIMP_TAC (list_ss++pred_setSimps.PRED_SET_ss++boolSimps.LIFT_COND_ss++boolSimps.EQUIV_EXTRACT_ss) []
+  rw[]
+
+    eq_tac >-(
+    rpt strip_tac
+    Q.EXISTS_TAC `Tev`
+    ASM_SIMP_TAC (srw_ss()) []
+    metis_tac[PTransEq]
+    )
+   rpt strip_tac
+   ASM_SIMP_TAC (srw_ss()) []
+    metis_tac[TreeTransEq]
+
+
+
+
+
+
+
+∀Tev T0 Tree. Tev ∈ (traces_of_tree T0 Tree) ⇒
+(∃Pev Re0 NRe0 Pro i Re NRe. (Pev ∈ (traces_of_sapic (Pconfig ((symbtree_to_sapic T0),0,Re0,NRe0)) (Pconfig (Pro,i,Re,NRe)))) ∧ (sim T0 (Pconfig ((symbtree_to_sapic T0),0,Re0,NRe0))) ⇒
+(trace_sim Tev Pev)
+)
+
+rewrite_tac[trace_sim_def]>>
+rewrite_tac[traces_of_sapic_def]>>
+rewrite_tac[traces_of_tree_def]>>
+ FULL_SIMP_TAC (list_ss++pred_setSimps.PRED_SET_ss++boolSimps.LIFT_COND_ss++boolSimps.EQUIV_EXTRACT_ss) []>>
+ gen_tac>>
+Cases_on ‘Tev’>-(
+rw[ execute_symbolic_tree_def]>>
+    Q.EXISTS_TAC `[]` >>
+    Q.EXISTS_TAC `Re0` >>
+    Q.EXISTS_TAC `NRe0` >>
+    Q.EXISTS_TAC `symbtree_to_sapic T0` >>
+    Q.EXISTS_TAC `0` >>
+    Q.EXISTS_TAC `Re0` >>
+    Q.EXISTS_TAC `NRe0` >>
+    rw[sapic_position_multi_transitions_def]>>
+    Q.EXISTS_TAC `T0` >>
+    Q.EXISTS_TAC `symbtree_to_sapic T0` >>
+    Q.EXISTS_TAC `0` >>
+    Q.EXISTS_TAC `Re0` >>
+    Q.EXISTS_TAC `NRe0` >>
+    ASM_SIMP_TAC (srw_ss()) []
+    )
+ rpt strip_tac
+ IMP_RES_TAC  execute_symbolic_tree_def
+ FULL_SIMP_TAC (list_ss++pred_setSimps.PRED_SET_ss++boolSimps.LIFT_COND_ss++boolSimps.EQUIV_EXTRACT_ss) []
+ Q.EXISTS_TAC `(pe::pev)` >>
+    Q.EXISTS_TAC `Re0` >>
+    Q.EXISTS_TAC `NRe0` >>
+    Q.EXISTS_TAC `Pro` >>
+    Q.EXISTS_TAC `i` >>
+    Q.EXISTS_TAC `Re` >>
+    Q.EXISTS_TAC `NRe` >>
+    rw[sapic_position_multi_transitions_def]
+ *)      
   
 val _ = export_theory();
